theories/language/adequacy.v
@@ -23,15 +23,8 @@ Definition zebre_adequacy Σ `{zebre_Gpre : !ZebreGpre Σ} e σ ϕ :
   adequate NotStuck e σ (λ v σ, ϕ v).
 Proof.
   intros Hwp.
-  apply adequate_alt. intros t2 σ2 (n & (κ & ?))%erased_steps_nsteps.
-  eapply (wp_strong_adequacy Σ _); last done.
-  iIntros "%Hinv_G".
-  iMod zebre_init as "(%zebre_G & Hsi)".
-  iDestruct (Hwp (Build_ZebreG Σ)) as "Hwp".
-  iModIntro.
-  iExists zebre_state_interp, [(λ v, ⌜ϕ v⌝%I)], (λ _, True%I), _ => /=.
-  iFrame. iStep. iIntros (es' t2' -> Hes' Hnot_stuck) " _ Hϕ _".
-  iApply fupd_mask_intro_discard; first done. iSplit; last done.
-  iDestruct (big_sepL2_cons_inv_r with "Hϕ") as (e' ? ->) "(Hϕ & _)".
-  iIntros (v2 t2'' [= -> <-]). rewrite to_of_val //.
+  apply: wp_adequacy => Hinv_G κs.
+  iMod zebre_init as "(%zebre_G & Hσ)".
+  iExists zebre_state_interp, (λ _, True%I). iFrame.
+  iApply (Hwp (Build_ZebreG Σ)).
 Qed.
